src/tactic/interactive.lean
@@ -835,17 +835,17 @@ propagate_tags $ ns.reverse.mmap' $ λ n, get_local n >>= tactic.revert_deps
 meta def revert_after (n : parse ident) : tactic unit :=
 propagate_tags $ get_local n >>= tactic.revert_after >> skip
 
-/-- `clearbody n₁ n₂ ...` clears the bodies of the local definitions `n₁, n₂ ...`, changing them
+/-- `clear_value n₁ n₂ ...` clears the bodies of the local definitions `n₁, n₂ ...`, changing them
   into regular hypotheses. A hypothesis `n : α := t` is changed to `n : α`. -/
-meta def clearbody (ns : parse ident*) : tactic unit :=
-propagate_tags $ ns.reverse.mmap' $ λ n, get_local n >>= tactic.clearbody
+meta def clear_value (ns : parse ident*) : tactic unit :=
+propagate_tags $ ns.reverse.mmap' $ λ n, get_local n >>= tactic.clear_value
 
 /--
 `generalize' : e = x` replaces all occurrences of `e` in the target with a new hypothesis `x` of the same type.
 
 `generalize' h : e = x` in addition registers the hypothesis `h : e = x`.
 
-`generalize'` is similar to `generalize`. The difference is that `generalize'` also succeeds when `e`
+`generalize'` is similar to `generalize`. The difference is that `generalize' : e = x` also succeeds when `e`
   does not occur in the goal. It is similar to `set`, but the resulting hypothesis `x` is not a local definition.
 -/
 meta def generalize' (h : parse ident?) (_ : parse $ tk ":") (p : parse generalize_arg_p) : tactic unit :=
